examples/formal-languages/regular/automata-tutorial/src/Summary.md
@@ -3,6 +3,7 @@
 [Introduction](README.md)
 
 - [Automata Definitions](./definitions.md)
-- [Subset Construction](./nfa-to-dfa.md)
-- [Transform a DFA to an NFA](./dfa-to-nfa.md)
+- [NFA to DFA](./nfa-to-dfa.md)
+- [DFA to NFA](./dfa-to-nfa.md)
 - [Final Result](./final-result.md)
+- [Exercises](./exercises.md)
