examples/formal-languages/regular/automata-tutorial/src/definitions.md
@@ -1,36 +1,30 @@
 # Automata
 
-Finite state automata are a core component of computer science. One of
-the nice things about them is their generality: automata appear in all
-kinds of places, and the ideas developed in automata theory permeate
-computer science.
-
 An automaton processes a *word*, a list of symbols drawn from an
-alphabet.  Processing goes symbol-by-symbol from left to right through
-the word. At each step the automaton is in a *state* and it
-transitions to a new state when it reads the next symbol. Once the
-word has been fully traversed the automaton decides whether to accept
-or reject the word; this is done by looking to see if the end state is
-an accepting one or not. So: from one view this is a perfectly
-mechanical process, but an automaton can also be viewed
-mathematically as implementing a *set*, namely the set of words that
-it accepts. The following formalization makes these ideas precise.
+*alphabet*. (Basically a word is a string, although it may draw from a
+non-traditional set of symbols.) Processing goes symbol-by-symbol from
+left to right through the word. At each step the automaton is in a
+*state* and it transitions to a new state when it reads the next
+symbol. Once the word has been fully traversed the automaton decides
+whether to accept or reject the word; this is done by looking to see
+if the current state is an *accepting* one or not.
 
-For this exercise we have a very simple notion of state: a state is
+For this tutorial we have a very simple notion of state: a state is
 just a natural number.
 
 ```
 Type state = “:num”
 ```
-Well, one might think so ... there are shenanigans to be played!
 
 ## Deterministic Finite-State Automata (DFAs)
 
-In textbooks, a DFA is defined to be a 5-tuple
-\\(\langle Q,\Sigma,\delta,S,F \rangle \\), where *Q* is a finite set of states,
-\\(\Sigma\\) is a finite set of symbols from which *words* may be formed,
-\\(\delta\\) is a transition function, *S* is the start state, and *F* is
-a set of final states.
+The above describes a *deterministic* automaton: given its current
+state and input symbol, there is one and only one next state it can go
+to. Formally, a DFA is defined to be a 5-tuple \\(\langle Q,\Sigma,\delta,S,F
+\rangle \\), where *Q* is a finite set of states, \\(\Sigma\\) is a
+finite set of symbols from which *words* may be formed, \\(\delta\\)
+is a transition function, *S* is the start state, and *F* is a set of
+final states. This 5-tuple is modelled by a record with 5 fields:
 
 ```
 Datatype:
@@ -44,17 +38,24 @@ Datatype:
 End
 ```
 
-DFA evaluation is defined by recursion:
+DFA evaluation is defined by recursion on the word:
 
 ```
 Definition dfa_eval_def:
-  dfa_eval N q [] = q ∧
-  dfa_eval N q (a::w) = dfa_eval N (N.delta q a) w
+  dfa_eval M q [] = q ∧
+  dfa_eval M q (a::w) = dfa_eval M (M.delta q a) w
 End
 ```
 
-The notion of *well-formedness* is important since the proofs we want
-to make depend on DFAs having certain properties:
+Evaluation iterates through the list of symbols, updating the state
+(variable *q*) for each symbol seen, and returning the state the
+machine is in once the end of the word is encountered. Notice that the
+definition of evaluation makes no mention of start states or final
+states. Those components come in when automata are treated as ways to
+compute sets.
+
+A notion of well-formedness of DFAs is also needed since not all possible
+values of the `dfa` type make sense.
 
 ```
 Definition wf_dfa_def:
@@ -67,9 +68,29 @@ Definition wf_dfa_def:
 End
 ```
 
+A wellformed DFA must have a finite set of states and the words it
+processes must be built from its (finite) alphabet. The other
+constraints imply that a well-formed DFA never strays outside of its
+state set.
+
+> [!WARNING]
+> `M.delta` is a HOL function, therefore it is a total function.  That
+> means that `M.delta q a` has a value for every possible `q` and `a`,
+> including, for example, when `q` is not in `M.Q` or `a` is
+> not in `M.Sigma`. In such situations the value of `M.delta q a`
+> exists, but all we really know about it is that it has type
+> `:num`. We are only assured that `M.delta q a` is a state of `M`
+> when `q` is a state of `M` and `a` is a symbol in the alphabet of
+> `M`. In short, one only wants to reason about applications of
+> `M.delta` in settings where it is known that `M` is a wellformed
+> DFA running on a word formed from `M.Sigma`.
+
+
 ## Non-deterministic Finite-State Automata (NFAs)
 
-NFAs have the same rough structure as DFAs, except that
+There are also *non-deterministic* automata: ones where, at each step
+of processing, there is a *set* of possible next states.  NFAs have much
+the same structure as DFAs, except that
 
 - the start states are a set
 - a transition results in a set of successor states
@@ -77,23 +98,47 @@ NFAs have the same rough structure as DFAs, except that
 ```
 Datatype:
   nfa = <|
-    Q : state set ;
-    Sigma : 'a set ;
-    delta : state -> 'a -> state set;
+    Q       : state set ;
+    Sigma   : 'a set ;
+    delta   : state -> 'a -> state set;
     initial : state set;
-    final : state set
+    final   : state set
   |>
 End
 ```
 
-NFA evaluation is defined by recursion:
+NFA evaluation is defined by recursion on the word argument.  A step
+of NFA evaluation `Delta N qset a` moves from the (possibly empty) set
+of states \\(\mathit{qset} = \\{q_1, \ldots, q_n\\} \\) to a successor
+set of states by
+
+1. For each \\(q_i \in \\mathit{qset}\\), an `M.delta` step is made on
+   symbol `a`, delivering a finite set of \\(q_i\\)-successors.
+
+2. This gives a set of sets which all get unioned together:
+\\[
+ M.delta\\; q_1 \\; a \cup \ldots\cup  M.delta\\; q_n\\; a
+\\]
+
+```
+Definition Delta_def:
+  Delta N qset a = BIGUNION{N.delta q a | q | q ∈ qset}
+End
+```
+
+We can think about NFA evaluation as evolving the fringe of a tree
+where the fringe at each step of evaluation represents the states that
+the machine might be in.
 
 ```
 Definition nfa_eval_def:
   nfa_eval N qset [] = qset ∧
-  nfa_eval N qset (a::w) = nfa_eval N (BIGUNION{N.delta q a | q | q ∈ qset}) w
+  nfa_eval N qset (a::w) = nfa_eval N (Delta N qset a) w
 End
 ```
+
+A wellformed NFA obeys ostensibly similar requirements as a wellformed
+DFA, adjusting for its usage of sets of states.
 
 ```
 Definition wf_nfa_def:
@@ -105,3 +150,71 @@ Definition wf_nfa_def:
     (∀q a. a ∈ N.Sigma ∧ q ∈ N.Q ⇒ N.delta q a ⊆ N.Q)
 End
 ```
+
+> [!NOTE]
+> The definition of wellformedness for NFAs allows the states of the
+> machine and the alphabet to be empty. The initial and final states
+> can also be empty, and the transition function could return an empty
+> set for every input, including well-formed ones. Indeed the
+> following theorem is straightforward:
+>
+> ```
+> Theorem wf_nfa_vacuous:
+>   wf_nfa <|
+>     Q       := ∅ ;
+>     Sigma   := ∅ ;
+>     delta   := λq a. ∅ ;
+>     initial := ∅ ;
+>     final   := ∅
+>   |>
+> Proof
+>   simp [wf_nfa_def]
+> QED
+> ```
+>
+> In contrast, a wellformed DFA has to have an initial state, so it
+> has at least one state, and every state must provide a transition to
+> a next state for every symbol in the alphabet.
+
+
+## Automata and Languages
+
+The execution of an automaton is a perfectly mechanical process, but
+an automaton can also be viewed mathematically as implementing a
+*set*, namely the set of words that it *accepts*. This is called the
+*language* of the automaton. A DFA `M` accepts word `w` if
+
+- `w` is built solely from `M.Sigma` symbols, and
+
+- execution on `w` starts in state `M.initial` and ends in one of the
+  states in `M.final`.
+
+```
+Definition dfa_lang_def:
+  dfa_lang M = {w | EVERY M.Sigma w ∧ dfa_eval M M.initial w ∈ M.final}
+End
+```
+
+An NFA `N` accepts word `w` if `w` is a word drawn from `N.Sigma` and
+execution on `w` starts with the set of states `N.initial` and ends in
+a set of states with a non-empty overlap with `M.final`.
+
+```
+Definition nfa_lang_def:
+  nfa_lang N = {w | EVERY N.Sigma w ∧ nfa_eval N N.initial w ∩ N.final ≠ ∅}
+End
+```
+
+We are now able to capture the languages implementable by DFAs and NFAs:
+
+```
+Definition DFA_LANGS_def:
+   DFA_LANGS = {dfa_lang M | wf_dfa M}
+End
+
+Definition NFA_LANGS_def:
+   NFA_LANGS = {nfa_lang N | wf_nfa N}
+End
+```
+
+We will show how to prove these are the same in the following sections.
