examples/formal-languages/regular/automata-tutorial/src/exercises.md
@@ -1,0 +1,47 @@
+# Exercises
+
+1. Formulate and prove the following statement of the Axiom of Choice:
+   *For every set of non-empty sets there exists a function that picks an
+   element from each set*.
+
+1. Make the type of "sets of states" into something that can be
+   computed over (lists, for example) and re-do the proofs.
+
+1. Another way to approach this material---in fact the standard
+   way---is to base it on *execution traces*. Say that a list of states
+   \\( [q_0, \\ldots q_n ] \\) is an NFA execution trace for *N* on
+   word *w* if it starts in a state of `N` and \\(q_{i+1} \in
+   M.delta\\; q_i \\; w_i \\) holds for each \\(i \in \\{0, \ldots,
+   |w| - 1 \\} \\).  This can be formulated as a recursive definition
+   in the following way:
+
+   ```
+   Definition nfa_trace_def:
+     nfa_trace N [q] [] = (q ∈ N.Q) ∧
+     nfa_trace N (q1::q2::t) (a::w) =
+        (a ∈ N.Sigma ∧
+         q1 ∈ N.Q ∧
+         q2 ∈ N.delta q1 a ∧
+         nfa_trace N (q2::t) w) ∧
+     nfa_trace N _ _ = F
+   End
+   ```
+
+   Then we can define the accepting traces of NFA `M` and the set of words having an accepting `N`-trace as follows:
+
+   ```
+   Definition accepting_nfa_trace_def:
+     accepting_nfa_trace N qs w <=>
+        nfa_trace N qs w ∧
+        HD qs ∈ N.initial ∧
+        LAST qs ∈ N.final
+   End
+
+   Definition nfa_trace_lang_def:
+     nfa_trace_lang N = {w | ∃qs. accepting_nfa_trace N qs w}
+   End
+   ```
+
+   Show that `nfa_trace_lang M = nfa_lang M`.
+
+1. Re-do the previous exercise, but use the `Inductive ... End` form to define the `nfa_trace` concept.
