examples/formal-languages/regular/automata-tutorial/src/nfa-to-dfa.md
@@ -1,32 +1,326 @@
-# Subset Construction
+# NFA to DFA
 
 A classic result of computer science theory is that the languages
 recognized by DFAs are equal to the languages recognized by NFAs. This
-was first proved by Dana Scott and Michael Rabin. The *subset
-construction* forms the backbone of the proof; it works by mapping an
-NFA into a dfa over subsets of the state space. In other words: a
-state of the constructed DFA embodies the states the NFA could
-possibly be in.
+was first proved by Michael Rabin and Dana Scott in *Finite automata
+and their decision problems*, IBM Journal of Research and Development
+3(2), 114–125 (1959).  The *subset construction* forms the backbone of
+their proof; it works by mapping an NFA into an "equivalent" DFA.
+
+The key insight is to make a state of the constructed DFA embody the
+states the NFA could possibly be in at a particular stage of
+processing the input word. The construction is conceptually appealing
+but it raises a technical problem: how to somehow arrange
+that the DFA state (a thing of type `:num`) *is* a set of NFA states
+(a thing of type `:num -> bool`). This cannot be accepted by the type
+system of HOL.
 
 ## Encoding subsets
 
-```
-(*===========================================================================*)
-(* The subset construction translates an NFA to a DFA. This relies on a      *)
-(* bijective mapping between sets of states and states.                      *)
-(*===========================================================================*)
+Our solution to the problem is to adopt a bijective mapping encoding
+sets of NFA states as natural numbers. Then we can arrange matters by
+defining the DFA so that its states are encodings of sets of NFA
+states. Thus we want two functions
 
+```
+  encode : num set -> num
+  decode : num -> num set
+```
+
+such that `decode (encode s) = s`. There is a variety of ways to
+achieve this; we choose one that highlights a distinctive aspect of
+the HOL logic, namely the *Hilbert Choice* operator.
+
+The Hilbert choice operator, written `@x. P x`, is syntax for
+expressing the notion "pick an *x* having property *P*".  (The Hilbert
+choice operator is also called the *Select* operator or even the
+*Indefinite description* operator.) The Choice operator is a way to
+form a term---intended to have a given property---in a context where
+that property may not in fact hold. The expectation is that, in a
+later, richer, context, the property will hold, and then the term can
+be reasoned with.
+
+This may sound like preposterous gobbledygook, so let's look at our
+desired encode/decode pair. First we define the encoder for an NFA `N`
+by picking a function `f` that is a bijection from the powerset `POW
+N.Q` of the states of `N` to a suitable set of numbers.
+
+```
 Definition encode_def:
   encode N = @f. ∃b. BIJ f (POW N.Q) (count b)
 End
+```
 
+In general such an `f` doesn't exist. (Why?) But it does if `N` is a
+wellformed NFA, since then `N.Q` is finite and so the powerset of
+states is finite. But before we get to that reasoning we are also able
+to define the decoder function as the left inverse to the encoder:
+
+```
 Definition decode_def:
   decode N = LINV (encode N) (POW N.Q)
 End
 ```
 
+We now create a context in which an encoder exists, and then our
+desired property can be proved:
 
-## Mapping to a DFA
+```
+Theorem codec:
+  wf_nfa N ∧ s ⊆ N.Q ⇒ decode N (encode N s) = s
+Proof
+  strip_tac >> simp [decode_def,encode_def] >>
+  SELECT_ELIM_TAC >> rw []
+  >- metis_tac [FINITE_BIJ_COUNT, BIJ_SYM, wf_nfa_def, FINITE_POW] >>
+  rename1 ‘BIJ f _ _’ >>
+  irule LINV_DEF >> metis_tac [IN_POW,BIJ_DEF]
+QED
+```
+
+We will look at this proof in detail.
+
+### Proofs with Hilbert's Choice terms
+
+To the initial goal we apply `strip_tac` which yields the goal
+
+```
+    0.  wf_nfa N
+    1.  s ⊆ N.Q
+   ------------------------------------
+        decode N (encode N s) = s
+```
+
+We bravely expand the definitions of both encoder and decoder:
+
+```
+  simp [decode_def,encode_def]
+```
+
+only to be confronted by a horrible-looking goal:
+
+```
+    0.  wf_nfa N
+    1.  s ⊆ N.Q
+   ------------------------------------
+        LINV (@f. ∃b. BIJ f (POW N.Q) (count b)) (POW N.Q)
+          ((@f. ∃b. BIJ f (POW N.Q) (count b)) s) =
+        s
+```
+
+The definition of `encode` has been expanded twice. (So we get two
+copies of the "choice" term.) Although this looks daunting, there is a
+useful tactic for goals with Hilbert choice terms:
+
+```
+  SELECT_ELIM_TAC
+```
+
+application of which generates a much nicer goal:
+
+```
+    0.  wf_nfa N
+    1.  s ⊆ N.Q
+   ------------------------------------
+        (∃x b. BIJ x (POW N.Q) (count b)) ∧
+        ∀x. (∃b. BIJ x (POW N.Q) (count b)) ⇒ LINV x (POW N.Q) (x s) = s
+```
+
+What has happened? We can make sense of it by looking at the theorem
+that `SELECT_ELIM_TAC` automates:
+
+```
+  > SELECT_ELIM_THM;
+  val it = ⊢ ∀P Q. (∃x. P x) ∧ (∀x. P x ⇒ Q x) ⇒ Q ($@ P): thm
+```
+
+This effectively reduces reasoning that a choice term `@x. P x` has
+property `Q` to two properties where the choice term is no longer
+present:
+
+- showing there is a witness for property `P`
+
+- showing that anything having property `P` also has property `Q`
+
+Returning to the proof, we split into two goals:
+
+```
+  rw []
+```
+
+This gives
+
+```
+    0.  wf_nfa N
+    1.  s ⊆ N.Q
+    2.  BIJ x (POW N.Q) (count b)
+   ------------------------------------
+        LINV x (POW N.Q) (x s) = s
+
+    0.  wf_nfa N
+    1.  s ⊆ N.Q
+   ------------------------------------
+        ∃x b. BIJ x (POW N.Q) (count b)
+```
+
+The lower goal goes first. We now search for any theorem that could
+help advance the proof. One can search by name or pattern; here we
+search for any theorem stored under a name including both `BIJ` and
+`count`. In fact the search term is `"bij~count"` since name search is
+case-insensitive. (The middle `~` symbol means that order is not
+relevant.) There are 4 results returned:
+
+```
+pred_setTheory.BIJ_NUM_COUNTABLE (THEOREM)
+------------------------------------------
+⊢ ∀s. (∃f. BIJ f 𝕌(:num) s) ⇒ countable s
+[$(HOLDIR)/src/pred_set/src/pred_setScript.sml:8710]
+
+
+pred_setTheory.COUNTABLE_ALT_BIJ (THEOREM)
+------------------------------------------
+⊢ ∀s. countable s ⇔ FINITE s ∨ BIJ (enumerate s) 𝕌(:num) s
+[$(HOLDIR)/src/pred_set/src/pred_setScript.sml:8728]
+
+
+pred_setTheory.FINITE_BIJ_COUNT (THEOREM)
+-----------------------------------------
+⊢ ∀s. FINITE s ⇒ ∃f b. BIJ f (count b) s
+[$(HOLDIR)/src/pred_set/src/pred_setScript.sml:4631]
+
+
+pred_setTheory.FINITE_BIJ_COUNT_EQ (THEOREM)
+--------------------------------------------
+⊢ ∀s. FINITE s ⇔ ∃c n. BIJ c (count n) s
+[$(HOLDIR)/src/pred_set/src/pred_setScript.sml:4613]
+```
+
+The last two are both usable. Let's work with `FINITE_BIJ_COUNT`.  One
+can reason as follows: "if `POW N.Q` is finite the theorem gives me a
+bijection `f` from a `count` set to it. But I actually need a
+bijection in the other direction, which I can get via `BIJ_SYM`". The
+details of this become tedious (try it) but a call to `metis_tac`
+automates the proof:
+
+```
+  metis_tac [FINITE_BIJ_COUNT, BIJ_SYM, wf_nfa_def, FINITE_POW]
+```
+
+The first conjunct is done. This leaves the goal
+
+```
+    0.  wf_nfa N
+    1.  s ⊆ N.Q
+    2.  BIJ x (POW N.Q) (count b)
+   ------------------------------------
+        LINV x (POW N.Q) (x s) = s
+```
+
+We can rename `x` to the more evocative `f` by giving a pattern:
+
+```
+  rename1 ‘BIJ f _ _’
+```
+
+This gives
+
+```
+    0.  wf_nfa N
+    1.  s ⊆ N.Q
+    2.  BIJ f (POW N.Q) (count b)
+   ------------------------------------
+        LINV f (POW N.Q) (f s) = s
+```
+
+A search with the pattern `LINV _ _ _ = _` finds two matching
+candidates, one of which is perfect:
+
+```
+pred_setTheory.LINV_DEF (THEOREM)
+---------------------------------
+⊢ ∀f s t. INJ f s t ⇒ ∀x. x ∈ s ⇒ LINV f s (f x) = x
+[$(HOLDIR)/src/pred_set/src/pred_setScript.sml:2785]
+```
+
+Backchaining with this theorem
+
+```
+  irule LINV_DEF
+```
+
+we obtain the goal
+
+```
+    0.  wf_nfa N
+    1.  s ⊆ N.Q
+    2.  BIJ f (POW N.Q) (count b)
+   ------------------------------------
+        s ∈ POW N.Q ∧ ∃t. INJ f (POW N.Q) t
+```
+
+Both conjuncts of this are direct consequences of the hypotheses
+and existing facts so we appeal to `metis_tac`:
+
+```
+  metis_tac [IN_POW,BIJ_DEF]
+```
+
+This succeeds, `metis_tac` printing some progress information as it
+works, and then the proof unwinds, proving intermediate goals back to
+the original goal.
+
+```
+metis: r[+0+10]+0+0+0+0+0+0+0+0+1#
+r[+0+10]+0+0+0+0+0+1#
+
+Goal proved.
+ [...] ⊢ s ∈ POW N.Q ∧ ∃t. INJ f (POW N.Q) t
+
+Goal proved.
+ [...] ⊢ LINV f (POW N.Q) (f s) = s
+
+Goal proved.
+ [...] ⊢ LINV x (POW N.Q) (x s) = s
+val it =
+   Initial goal proved.
+   ⊢ wf_nfa N ∧ s ⊆ N.Q ⇒ decode N (encode N s) = s: proof
+>
+```
+
+That finishes the proof.
+
+> [!NOTE]
+> Our usage of the Select operator is motivated by wanting a compact
+> formulation of encoding/decoding free of algorithmic details. In HOL
+> we can simply "pick a suitable bijection" and quickly derive the
+> invertibility result needed. It is, however, non-constructive: a
+> computable implementation would require a concrete datatype such as
+> lists or trees to represent state sets.
+
+> [!NOTE]
+> Our usage of Hilbert choice in this example amounts to a
+> kind of "eliminable but convenient" shorthand for some messier
+> reasoning. However the Choice operator can do much more: the full
+> power of the Axiom of Choice is available in HOL in the form of
+> the following axiom:
+>
+> ```
+> SELECT_AX;
+> val it = ⊢ ∀P x. P x ⇒ P ($@ P): thm
+> ```
+
+
+### Abbreviating encode/decode
+
+We establish `enc` and `dec` as abbreviations for `encode N` and
+`decode N`, using the following declarations:
+
+```
+Overload "enc"[local] = “encode N”
+Overload "dec"[local] = “decode N”;
+```
+
+
+## The subset construction
 
 The construction maps an NFA structure to a DFA structure, using the
 encoder to collapse subsets to states and the decoder to recover
@@ -37,12 +331,20 @@ Definition nfa_to_dfa_def:
   nfa_to_dfa N : 'a dfa =
     <| Q       := {enc s | s | s ⊆ N.Q};
        Sigma   := N.Sigma;
-       delta   := λqs a. enc (BIGUNION {N.delta q a | q | q ∈ dec qs});
+       delta   := λqs a. enc (Delta N (dec qs) a);
        initial := enc N.initial;
        final   := {enc s | s | s ⊆ N.Q ∧ s ∩ N.final ≠ ∅}
     |>
 End
 ```
+
+Thus the set of states of the constructed DFA is the set of encodings
+of all subsets of the NFA state set. The initial state is the encoding
+of the initial states of the NFA. The final states are the encodings
+of any subsets of the state space of the NFA that have at least one
+final state.  Finally, a computation step in the DFA takes the current
+state, decodes it to a set of NFA states, runs the NFA `Delta`, and
+encodes the result.
 
 The key lemma about the construction is the following:
 
@@ -61,6 +363,9 @@ Proof
   DEP_REWRITE_TAC [codec] >> simp []
 QED
 ```
+
+This expresses a kind of commutative diagram.
+
 
 And then we can prove one direction of the final result:
 
